Make Read and Write type classes

nola/examples/rust_halt/ptr.v
@@ -43,53 +43,38 @@ Section read_write.
   Context `{!rust_haltGS CON Σ, rust_haltJ CON JUDG Σ, !Csem CON JUDG Σ,
     !Jsem JUDG (iProp Σ)}.
 
-  (** [read]: Read from a pointer type *)
-  Definition read_def {X Y X'} (α : lft) (T : ty CON Σ X) (U : ty CON Σ Y)
-    (T' : ty CON Σ X') (get : X → Y) (set : X → X') : iProp Σ :=
-    □ ∀ q t d xπ v, q.[α] -∗ na_own t ⊤ -∗ ⟦ T.1 t d xπ [v] ⟧ᶜ
-      =[rust_halt_wsat]{⊤}=∗ ∃ l wl du r,
-        ⌜v = # l⌝ ∗ l ↦∗{r} wl ∗ ⟦ U.1 t du (get ∘ xπ) wl ⟧ᶜ ∗
-        (l ↦∗{r} wl =[rust_halt_wsat]{⊤}=∗ ∃ d',
-          q.[α] ∗ na_own t ⊤ ∗ ⟦ T'.1 t d' (set ∘ xπ) [v] ⟧ᶜ).
-  Lemma read_aux : seal (@read_def). Proof. by eexists _. Qed.
-  Definition read {X Y X'} := read_aux.(unseal) X Y X'.
-  Lemma read_unseal : @read = @read_def. Proof. by exact: seal_eq. Qed.
+  (** [Read]: Read from a pointer type *)
+  Class Read {X Y X'} (α : lft) (T : ty CON Σ X) (U : ty CON Σ Y)
+    (T' : ty CON Σ X') (get : X → Y) (set : X → X') : Prop := READ {
+    read {q t d xπ v} :
+      q.[α] -∗ na_own t ⊤ -∗ ⟦ T.1 t d xπ [v] ⟧ᶜ =[rust_halt_wsat]{⊤}=∗
+        ∃ l wl du r, ⌜v = # l⌝ ∗ l ↦∗{r} wl ∗ ⟦ U.1 t du (get ∘ xπ) wl ⟧ᶜ ∗
+          (l ↦∗{r} wl =[rust_halt_wsat]{⊤}=∗ ∃ d',
+            q.[α] ∗ na_own t ⊤ ∗ ⟦ T'.1 t d' (set ∘ xπ) [v] ⟧ᶜ);
+  }.
 
-  (** [read] is persistent *)
-  #[export] Instance read_persistent {X Y X' α T U T' get set} :
-    Persistent (@read X Y X' α T U T' get set).
-  Proof. rewrite read_unseal. exact _. Qed.
-
-  (** [write]: Write to a pointer type *)
-  Definition write_def {X Y Y' X'} (α : lft) (T : ty CON Σ X) (U : ty CON Σ Y)
+  (** [Write]: Write to a pointer type *)
+  Class Write {X Y Y' X'} (α : lft) (T : ty CON Σ X) (U : ty CON Σ Y)
     (U' : ty CON Σ Y') (T' : ty CON Σ X') (get : X → Y) (set : X → Y' → X')
-    : iProp Σ :=
-    □ ∀ q t d xπ v, q.[α] -∗ ⟦ T.1 t d xπ [v] ⟧ᶜ
-      =[rust_halt_wsat]{⊤}=∗ ∃ l wl du,
+    : Prop := WRITE {
+    write {q t d xπ v} :
+      q.[α] -∗ ⟦ T.1 t d xπ [v] ⟧ᶜ =[rust_halt_wsat]{⊤}=∗ ∃ l wl du,
         ⌜v = # l⌝ ∗ l ↦∗ wl ∗ ⟦ U.1 t du (get ∘ xπ) wl ⟧ᶜ ∗
         (∀ du' yπ' wl', l ↦∗ wl' -∗ ⟦ U'.1 t du' yπ' wl' ⟧ᶜ
           =[rust_halt_wsat]{⊤}=∗ ∃ d',
-          q.[α] ∗ ⟦ T'.1 t d' (λ π, set (xπ π) (yπ' π)) [v] ⟧ᶜ).
-  Lemma write_aux : seal (@write_def). Proof. by eexists _. Qed.
-  Definition write {X Y Y' X'} := write_aux.(unseal) X Y Y' X'.
-  Lemma write_unseal : @write = @write_def. Proof. by exact: seal_eq. Qed.
-
-  (** [write] is persistent *)
-  #[export] Instance write_persistent {X Y Y' X' α T U U' T' get set} :
-    Persistent (@write X Y Y' X' α T U U' T' get set).
-  Proof. rewrite write_unseal. exact _. Qed.
+          q.[α] ∗ ⟦ T'.1 t d' (λ π, set (xπ π) (yπ' π)) [v] ⟧ᶜ);
+  }.
 
   (** Reading a value from a pointer *)
-  Lemma type_read
-    `{!EtcxExtract (X:=X) (Yl:=Zl) (Zl:=Zl') (v ◁ T) Γ Γr get' getr}
-    `{!Ty (X:=Y) U 1} {X' T' get set α} :
-    read (X':=X') α T U T' get set ⊢
-      type α Γ (!v) (λ r, r ◁ U ᵖ:: v ◁ T' ᵖ:: Γr)
-        (λ post zl, let x := get' zl in post (get x, set x, getr zl)').
+  Lemma type_read v
+    `{!EtcxExtract (X:=X) (Yl:=Zl) (Zl:=Zl') (v ◁ T) Γ Γr get' getr,
+      !Read (Y:=Y) (X':=X') α T U T' get set, !Ty U 1} :
+    ⊢ type α Γ (!v) (λ r, r ◁ U ᵖ:: v ◁ T' ᵖ:: Γr)
+      (λ post zl, let x := get' zl in post (get x, set x, getr zl)').
   Proof.
-    rewrite read_unseal type_unseal. iIntros "#read !>" (????) "α t pre".
+    rewrite type_unseal. iIntros (????) "!> α t pre".
     rewrite etcx_extract /=. iIntros "[[% T] Γr]".
-    iMod ("read" with "α t T") as (? wl ?? ->) "(↦ & U & →T')".
+    iMod (read with "α t T") as (? wl ?? ->) "(↦ & U & →T')".
     iDestruct (ty_own_size with "U") as %?. destruct wl as [|w[|??]]=>//.
     rewrite heap_pointsto_vec_singleton. wp_read.
     iMod ("→T'" with "↦") as (?) "($ & $ & T')". iModIntro. iFrame "pre".
@@ -97,17 +82,15 @@ Section read_write.
   Qed.
 
   (** Writing a value to a pointer *)
-  Lemma type_write
-    `{!TcxExtract (Xl:=[X;Y]) (Yl:=Zl) (Zl:=Zl') ᵖ[v ◁ T; w ◁ U] Γ Γr get' getr}
-    `{!Ty (X:=Y') U' 1} {X' T' get set α} :
-    write (Y:=Y') (X':=X') α T U' U T' get set ⊢
-      type α Γ (v <- w) (λ _, v ◁ T' ᵖ:: Γr)
+  Lemma type_write v w
+    `{!TcxExtract (Xl:=[X;Y]) (Yl:=Zl) (Zl:=Zl') ᵖ[v ◁ T; w ◁ U] Γ Γr get' getr,
+      !Write (Y:=Y') (X':=X') α T U' U T' get set, !Ty U' 1} :
+    ⊢ type α Γ (v <- w) (λ _, v ◁ T' ᵖ:: Γr)
         (λ post zl, let '(x, y, _)' := get' zl in post (set x y, getr zl)').
   Proof.
-    rewrite write_unseal type_unseal.
-    iIntros "#write !>" (????) "α $ pre". rewrite tcx_extract /=.
+    rewrite type_unseal. iIntros (????) "!> α $ pre". rewrite tcx_extract /=.
     iIntros "[([% T] & [% U] & _) Γr]".
-    iMod ("write" with "α T") as (? wl ? ->) "(↦ & U' & →T')".
+    iMod (write with "α T") as (? wl ? ->) "(↦ & U' & →T')".
     iDestruct (ty_own_size with "U'") as %?. destruct wl as [|?[|??]]=>//.
     rewrite heap_pointsto_vec_singleton. wp_write.
     rewrite -heap_pointsto_vec_singleton.
@@ -115,21 +98,19 @@ Section read_write.
   Qed.
 
   (** Memory copy *)
-  Lemma type_memcopy
+  Lemma type_memcopy vs vt
     `{!TcxExtract (Xl:=[Xs; Xt]) (Yl:=Zl) (Zl:=Zl') ᵖ[vs ◁ Ts; vt ◁ Tt] Γ Γr
-        get getr, !Ty (X:=Y) U sz, !Ty (X:=Y') U' sz}
-    {Xs' Ts' gets sets Xt' Tt' gett sett α} :
-    read (Y:=Y) (X':=Xs') α Ts U Ts' gets sets -∗
-    write (Y:=Y') (X':=Xt') α Tt U' U Tt' gett sett -∗
-      type α Γ (vt <-{sz} !vs)%E (λ _, vs ◁ Ts' ᵖ:: vt ◁ Tt' ᵖ:: Γr)
+        get getr,
+      !Read (Y:=Y) (X':=Xs') α Ts U Ts' gets sets,
+      !Write (Y:=Y') (X':=Xt') α Tt U' U Tt' gett sett, !Ty U sz, !Ty U' sz} :
+    ⊢ type α Γ (vt <-{sz} !vs)%E (λ _, vs ◁ Ts' ᵖ:: vt ◁ Tt' ᵖ:: Γr)
         (λ post zl, let '(xs, xt, _)' := get zl in
           post (sets xs, sett xt (gets xs), getr zl)').
   Proof.
-    rewrite read_unseal write_unseal type_unseal.
-    iIntros "#read #write !>" (????) "[α α'] t pre". rewrite tcx_extract /=.
-    iIntros "[([% Ts] & [% Tt] & _) Γr]".
-    iMod ("read" with "α t Ts") as (? wls ?? ->) "(↦s & U & →Ts')".
-    iMod ("write" with "α' Tt") as (? wlt ? ->) "(↦t & U' & →Tt')".
+    rewrite type_unseal. iIntros (????) "!> [α α'] t pre".
+    rewrite tcx_extract /=. iIntros "[([% Ts] & [% Tt] & _) Γr]".
+    iMod (read with "α t Ts") as (? wls ?? ->) "(↦s & U & →Ts')".
+    iMod (write with "α' Tt") as (? wlt ? ->) "(↦t & U' & →Tt')".
     iDestruct (ty_own_size with "U") as %?.
     iDestruct (ty_own_size with "U'") as %?.
     wp_apply (twp_memcpy wls wlt with "[$↦s $↦t]")=>//. iIntros "[↦s ↦t]".
